model fixed. Mediator function finalized

txn-data-consistency/CCv_Eiger_Port_modified.thy
@@ -8,9 +8,8 @@ subsection \<open>Event system & Refinement from ET_ES to tps\<close>
 
 subsubsection \<open>State\<close>
 
-typedecl svr_id
+type_synonym svr_id = key
 type_synonym tstmp = nat
-consts loc :: "key \<Rightarrow> svr_id" 
 
 record 'v ep_version = "'v version" +
   v_ts :: tstmp
@@ -24,18 +23,19 @@ definition ep_version_init :: "'v ep_version" where
     v_ts = 0, v_gst = 0, v_is_pending = False\<rparr>"
 
 \<comment> \<open>Server State\<close>
-datatype state_wtxn = Ready | Prep tstmp | Commit
-datatype state_rtxn = NotReg | Regd
+datatype state_wtxn = Ready | Prep tstmp v_id | Commit
 record 'v server =
-  wtxn_state :: "txid0 \<Rightarrow> key \<Rightarrow> state_wtxn"
-  rtxn_state :: "txid0 \<Rightarrow> key \<Rightarrow> state_rtxn"
+  wtxn_state :: "txid0 \<Rightarrow> state_wtxn"
   clock :: tstmp
   lst :: tstmp
   pending_wtxns :: "txid0 \<rightharpoonup> tstmp"
-  DS :: "'v datastore"
+  DS :: "'v ep_version list"
+
+definition DS_vl_init :: "'v ep_version list" where
+  "DS_vl_init \<equiv> [ep_version_init]"
 
 definition DS_init :: "'v datastore" where
-  "DS_init \<equiv> (\<lambda>k. [ep_version_init])"
+  "DS_init \<equiv> (\<lambda>k. DS_vl_init)"
 
 \<comment> \<open>Client State\<close>
 datatype 'v state_txn = Idle | RtxnInProg "key set" "key \<rightharpoonup> 'v" | WtxnPrep "key \<rightharpoonup> 'v" |
@@ -55,10 +55,37 @@ record 'v state =
 subsubsection \<open>Events\<close>
 
 datatype 'v ev =
-  RInvoke cl_id "key set" sqn view "'v fingerpr"| Read cl_id key 'v | RDone cl_id "key \<rightharpoonup> 'v" |
-  WInvoke cl_id "key \<rightharpoonup> 'v" | WCommit cl_id "key \<rightharpoonup> 'v" tstmp sqn view "'v fingerpr" | WDone cl_id |
-  RegR svr_id txid0 key 'v v_id tstmp | PrepW svr_id txid0 key 'v tstmp | CommitW svr_id txid0 key |
-  Skip2
+  RInvoke cl_id "key set" | Read cl_id key 'v | RDone cl_id "key \<rightharpoonup> 'v" sqn view |
+  WInvoke cl_id "key \<rightharpoonup> 'v" | WCommit cl_id "key \<rightharpoonup> 'v" tstmp sqn view | WDone cl_id |
+  RegR svr_id txid0 'v v_id tstmp | PrepW svr_id txid0 'v tstmp | CommitW svr_id txid0 | Skip2
+
+definition svr_t'_unchanged where
+  "svr_t'_unchanged t k s s' \<equiv> (\<forall>t'. t' \<noteq> t \<longrightarrow>
+    wtxn_state (svrs s' k) t' = wtxn_state (svrs s k) t' \<and>
+    pending_wtxns (svrs s' k) t' = pending_wtxns (svrs s k) t')"
+
+definition other_insts_unchanged where
+  "other_insts_unchanged e s s' \<equiv> (\<forall>e'. e' \<noteq> e \<longrightarrow> s' e' = s e')"
+
+definition cls_svr_k'_t'_unchanged where
+  "cls_svr_k'_t'_unchanged t k s s' \<equiv> cls s' = cls s \<and>
+    other_insts_unchanged k (svrs s) (svrs s') \<and> svr_t'_unchanged t k s s'"
+
+definition svrs_cls_cl'_unchanged where
+  "svrs_cls_cl'_unchanged cl s s' \<equiv> svrs s' = svrs s \<and> other_insts_unchanged cl (cls s) (cls s')"
+
+lemmas km_unchanged_defs = cls_svr_k'_t'_unchanged_def other_insts_unchanged_def svr_t'_unchanged_def
+lemmas tm_unchanged_defs = svrs_cls_cl'_unchanged_def other_insts_unchanged_def
+lemmas unchanged_defs = km_unchanged_defs svrs_cls_cl'_unchanged_def
+
+definition tid_match :: "'v state \<Rightarrow> txid0 \<Rightarrow> bool" where
+  "tid_match s t \<equiv> txn_sn (cls s (get_cl_txn t)) = get_sn_txn t"
+
+abbreviation add_to_readerset :: "'v ep_version list \<Rightarrow> txid0 \<Rightarrow> v_id \<Rightarrow> 'v ep_version list" where
+  "add_to_readerset vl t i \<equiv> vl [i := (vl ! i)\<lparr>v_readerset := insert t (v_readerset (vl ! i))\<rparr>]"
+
+abbreviation commit_in_vl :: "'v ep_version list \<Rightarrow> tstmp \<Rightarrow> v_id \<Rightarrow> 'v ep_version list" where
+  "commit_in_vl vl commit_t i \<equiv> vl [i := (vl ! i)\<lparr>v_ts := commit_t, v_is_pending := False\<rparr>]"
 
 abbreviation get_txn_cl :: "'v state \<Rightarrow> cl_id \<Rightarrow> txid0" where
   "get_txn_cl s cl \<equiv> Tn_cl (txn_sn (cls s cl)) cl"
@@ -85,21 +112,15 @@ definition read_at :: "'v ep_version list \<Rightarrow> tstmp \<Rightarrow> cl_i
       None \<Rightarrow> (v_value ver, i) | Some (ver', i') \<Rightarrow> (v_value ver', i'))"
 
 \<comment> \<open>Clint Events\<close>
-definition read_invoke :: "cl_id \<Rightarrow> key set \<Rightarrow> sqn \<Rightarrow> view \<Rightarrow> 'v fingerpr \<Rightarrow> 'v state \<Rightarrow> 'v state \<Rightarrow> bool" where
-  "read_invoke cl keys sn u F s s' \<equiv> 
-    sn = txn_sn (cls s cl) \<and>
-    u = cl_view (cls s cl) \<and>
-    (\<forall>k. F k W = None) \<and> (\<forall>k. k \<notin> keys \<longrightarrow> F k R = None) \<and>
-    (\<forall>k \<in> keys. \<exists>v i. F k R = Some v \<and>
-     (v, i) = read_at (rev (DS (svrs s (loc k)) k)) (gst (cls s cl)) cl \<and>
-     cl_view (cls s' cl) k = insert i (cl_view (cls s cl) k)) \<and>
+definition read_invoke :: "cl_id \<Rightarrow> key set \<Rightarrow> 'v state \<Rightarrow> 'v state \<Rightarrow> bool" where
+  "read_invoke cl keys s s' \<equiv>
     txn_state (cls s cl) = Idle \<and>
     txn_state (cls s' cl) = RtxnInProg keys (Map.empty) \<and>
     txn_sn (cls s' cl) = txn_sn (cls s cl) \<and>
     gst (cls s' cl) = max (gst (cls s cl)) (Min (range (lst_map (cls s cl)))) \<and>
     lst_map (cls s' cl) = lst_map (cls s cl) \<and>
-    (\<forall>k'. k' \<notin> keys \<longrightarrow> cl_view (cls s' cl)k' = cl_view (cls s cl) k') \<and>
-    svrs s' = svrs s"
+    cl_view (cls s' cl) = cl_view (cls s cl) \<and>
+    svrs_cls_cl'_unchanged cl s s'"
 
 fun find_and_read_val :: "'v ep_version list \<Rightarrow> txid0 \<rightharpoonup> 'v" where
   "find_and_read_val [] t = None" |
@@ -108,27 +129,30 @@ fun find_and_read_val :: "'v ep_version list \<Rightarrow> txid0 \<rightharpoonu
 
 definition read :: "cl_id \<Rightarrow> key \<Rightarrow> 'v \<Rightarrow> 'v state \<Rightarrow> 'v state \<Rightarrow> bool" where
   "read cl k v s s' \<equiv> \<exists>keys vals.
-    rtxn_state (svrs s (loc k)) (get_txn_cl s cl) k = Regd \<and>
-    Some v = find_and_read_val (rev (DS (svrs s (loc k)) k)) (get_txn_cl s cl) \<and>
+    Some v = find_and_read_val (rev (DS (svrs s k))) (get_txn_cl s cl) \<and>
     txn_state (cls s cl) = RtxnInProg keys vals \<and> k \<in> keys \<and> vals k = None \<and>
     txn_state (cls s' cl) = RtxnInProg keys (vals (k \<mapsto> v)) \<and>
     txn_sn (cls s' cl) = txn_sn (cls s cl) \<and>
     gst (cls s' cl) = gst (cls s cl) \<and>
-    lst_map (cls s' cl) (loc k) = lst (svrs s (loc k)) \<and>
-    (\<forall>l. l \<noteq> loc k \<longrightarrow> lst_map (cls s' cl) = lst_map (cls s cl)) \<and>
+    lst_map (cls s' cl) k = lst (svrs s k) \<and>
+    (\<forall>k'. k' \<noteq> k \<longrightarrow> lst_map (cls s' cl) k' = lst_map (cls s cl) k') \<and>
     cl_view (cls s' cl) = cl_view (cls s cl) \<and>
-    svrs s' = svrs s"
+    svrs_cls_cl'_unchanged cl s s'"
 
-definition read_done :: "cl_id \<Rightarrow> (key \<rightharpoonup> 'v) \<Rightarrow> 'v state \<Rightarrow> 'v state \<Rightarrow> bool" where
-  "read_done cl vals s s' \<equiv> (\<exists>keys.
-    txn_state (cls s cl) = RtxnInProg keys vals \<and> dom vals = keys \<and>
-    (\<forall>k\<in>keys. rtxn_state (svrs s (loc k)) (get_txn_cl s cl) k = Regd)) \<and>
+definition read_done :: "cl_id \<Rightarrow> (key \<rightharpoonup> 'v) \<Rightarrow> sqn \<Rightarrow> view \<Rightarrow> 'v state \<Rightarrow> 'v state \<Rightarrow> bool" where
+  "read_done cl kv_map sn u s s' \<equiv>
+    sn = txn_sn (cls s cl) \<and>
+    u = cl_view (cls s cl) \<and>
+    (\<forall>k \<in> dom kv_map. \<exists>v i.
+     (v, i) = read_at (rev (DS (svrs s k))) (gst (cls s cl)) cl \<and>
+     cl_view (cls s' cl) k = insert i (cl_view (cls s cl) k)) \<and>
+    (\<exists>keys. txn_state (cls s cl) = RtxnInProg keys kv_map \<and> dom kv_map = keys) \<and>
     txn_state (cls s' cl) = Idle \<and>
     txn_sn (cls s' cl) = Suc (txn_sn (cls s cl)) \<and>
     gst (cls s' cl) = gst (cls s cl) \<and>
     lst_map (cls s' cl) = lst_map (cls s cl) \<and>
-    cl_view (cls s' cl) = cl_view (cls s cl) \<and>
-    svrs s' = svrs s"
+    (\<forall>k. k \<notin> dom kv_map \<longrightarrow> cl_view (cls s' cl) k = cl_view (cls s cl) k) \<and>
+    svrs_cls_cl'_unchanged cl s s'"
 
 definition write_invoke :: "cl_id \<Rightarrow> (key \<rightharpoonup> 'v) \<Rightarrow> 'v state \<Rightarrow> 'v state \<Rightarrow> bool" where
   "write_invoke cl kv_map s s' \<equiv> 
@@ -139,98 +163,82 @@ definition write_invoke :: "cl_id \<Rightarrow> (key \<rightharpoonup> 'v) \<Rig
     gst (cls s' cl) = gst (cls s cl) \<and>
     lst_map (cls s' cl) = lst_map (cls s cl) \<and>
     cl_view (cls s' cl) = cl_view (cls s cl) \<and>
-    svrs s' = svrs s"
+    svrs_cls_cl'_unchanged cl s s'"
 
-definition write_commit :: "cl_id \<Rightarrow> (key \<rightharpoonup> 'v) \<Rightarrow> tstmp \<Rightarrow> sqn \<Rightarrow> view \<Rightarrow> 'v fingerpr \<Rightarrow> 'v state \<Rightarrow> 'v state \<Rightarrow> bool" where
-  "write_commit cl kv_map commit_t sn u F s s' \<equiv>
+definition write_commit :: "cl_id \<Rightarrow> (key \<rightharpoonup> 'v) \<Rightarrow> tstmp \<Rightarrow> sqn \<Rightarrow> view \<Rightarrow> 'v state \<Rightarrow> 'v state \<Rightarrow> bool" where
+  "write_commit cl kv_map commit_t sn u s s' \<equiv>
     sn = txn_sn (cls s cl) \<and>
     u = cl_view (cls s cl) \<and>
-    (\<forall>k. F k R = None) \<and> (\<forall>k. F k W = kv_map k) \<and>
     txn_state (cls s cl) = WtxnPrep kv_map \<and>
-    (\<forall>k \<in> dom kv_map. \<exists>prep_t.
-      wtxn_state (svrs s (loc k)) (get_txn_cl s cl) k = Prep prep_t) \<and>
-    commit_t = Max {prep_t. (\<exists>k \<in> dom kv_map.
-      wtxn_state (svrs s (loc k)) (get_txn_cl s cl) k = Prep prep_t)} \<and>
+    (\<forall>k \<in> dom kv_map. \<exists>prep_t i.
+      wtxn_state (svrs s k) (get_txn_cl s cl) = Prep prep_t i \<and>
+      cl_view (cls s' cl) k = insert i (cl_view (cls s cl) k)) \<and> \<comment> \<open>use Let\<close>
+    commit_t = Max {prep_t. (\<exists>k \<in> dom kv_map. \<exists>i.
+      wtxn_state (svrs s k) (get_txn_cl s cl) = Prep prep_t i)} \<and>
     txn_state (cls s' cl) = WtxnCommit commit_t kv_map \<and>
     txn_sn (cls s' cl) = txn_sn (cls s cl) \<and>
     gst (cls s' cl) = gst (cls s cl) \<and>
     lst_map (cls s' cl) = lst_map (cls s cl) \<and>
-    \<comment> \<open>update cl_view\<close>
-    svrs s' = svrs s"
+    (\<forall>k. k \<notin> dom kv_map \<longrightarrow> cl_view (cls s' cl) k = cl_view (cls s cl) k) \<and>
+    svrs_cls_cl'_unchanged cl s s'"
 
 definition write_done :: "cl_id \<Rightarrow> 'v state \<Rightarrow> 'v state \<Rightarrow> bool" where
   "write_done cl s s' \<equiv> \<exists>kv_map commit_t.
     txn_state (cls s cl) = WtxnCommit commit_t kv_map \<and>
-    (\<forall>k\<in>dom kv_map. wtxn_state (svrs s (loc k)) (get_txn_cl s cl) k = Commit) \<and>
+    (\<forall>k\<in>dom kv_map. wtxn_state (svrs s k) (get_txn_cl s cl) = Commit) \<and>
     txn_state (cls s' cl) = Idle \<and>
     txn_sn (cls s' cl) = Suc (txn_sn (cls s cl)) \<and>
     gst (cls s' cl) = gst (cls s cl) \<and>
-    (\<forall>l. l \<in> loc ` (dom kv_map) \<longrightarrow> lst_map (cls s' cl) l = lst (svrs s l)) \<and>
-    (\<forall>l. l \<notin> loc ` (dom kv_map) \<longrightarrow> lst_map (cls s' cl) l = lst_map (cls s cl) l) \<and>
+    (\<forall>k. k \<in> dom kv_map \<longrightarrow> lst_map (cls s' cl) k = lst (svrs s k)) \<and>
+    (\<forall>k. k \<notin> dom kv_map \<longrightarrow> lst_map (cls s' cl) k = lst_map (cls s cl) k) \<and>
     cl_view (cls s' cl) = cl_view (cls s cl) \<and>
-    svrs s' = svrs s"
+    svrs_cls_cl'_unchanged cl s s'"
 
 \<comment> \<open>Server Events\<close>
-definition register_read :: "svr_id \<Rightarrow> txid0 \<Rightarrow> key \<Rightarrow> 'v \<Rightarrow> v_id \<Rightarrow> tstmp \<Rightarrow> 'v state \<Rightarrow> 'v state \<Rightarrow> bool" where
-  "register_read svr t k v i gst_ts s s' \<equiv> \<exists>keys vals.
-    txn_state (cls s (get_cl_txn t)) = RtxnInProg keys vals \<and> k \<in> keys \<and> vals k = None \<and>
-    (v, i) = read_at (rev (DS (svrs s svr) k)) gst_ts (get_cl_txn t) \<and>
+definition register_read :: "svr_id \<Rightarrow> txid0 \<Rightarrow> 'v \<Rightarrow> v_id \<Rightarrow> tstmp \<Rightarrow> 'v state \<Rightarrow> 'v state \<Rightarrow> bool" where
+  "register_read svr t v i gst_ts s s' \<equiv>
+    tid_match s t \<and>
+    (\<exists>keys vals.
+      txn_state (cls s (get_cl_txn t)) = RtxnInProg keys vals \<and> svr \<in> keys \<and> vals svr = None) \<and>
+    (v, i) = read_at (rev (DS (svrs s svr))) gst_ts (get_cl_txn t) \<and>
     gst_ts = gst (cls s (get_cl_txn t)) \<and>
-    loc k = svr \<and>
-    rtxn_state (svrs s svr) t k = NotReg \<and>
-    rtxn_state (svrs s' svr) t k = Regd \<and>
-    (\<forall>t' k'. t' \<noteq> t \<or> k' \<noteq> k \<longrightarrow> rtxn_state (svrs s' svr) t' k' = rtxn_state (svrs s svr) t' k') \<and>
     wtxn_state (svrs s' svr) = wtxn_state (svrs s svr) \<and>
     clock (svrs s' svr) = Suc (clock (svrs s svr)) \<and>
     lst (svrs s' svr) = lst (svrs s svr) \<and>
     pending_wtxns (svrs s' svr) = pending_wtxns (svrs s svr) \<and>
-    DS (svrs s' svr) k = (DS (svrs s svr) k) [i :=
-      (DS (svrs s svr) k ! i)\<lparr>v_readerset := insert t (v_readerset (DS (svrs s svr) k ! i))\<rparr>] \<and>
-    (\<forall>k'. k' \<noteq> k \<longrightarrow> DS (svrs s' svr) k' = DS (svrs s svr) k') \<and>
-    cls s' = cls s"
+    DS (svrs s' svr) = add_to_readerset (DS (svrs s svr)) t i \<and>
+    cls_svr_k'_t'_unchanged t svr s s'"
 
-definition prepare_write :: "svr_id \<Rightarrow> txid0 \<Rightarrow> key \<Rightarrow> 'v \<Rightarrow> tstmp \<Rightarrow> 'v state \<Rightarrow> 'v state \<Rightarrow> bool" where
-  "prepare_write svr t k v gst_ts s s' \<equiv> \<exists>kv_map.
-    txn_state (cls s (get_cl_txn t)) = WtxnPrep kv_map \<and> k \<in> dom kv_map \<and> kv_map k = Some v \<and>
-    gst_ts =  (gst (cls s (get_cl_txn t))) \<and> 
-    loc k = svr \<and>
-    wtxn_state (svrs s svr) t k = Ready \<and>
-    wtxn_state (svrs s' svr) t k = Prep (clock (svrs s' svr)) \<and>
-    (\<forall>t' k'. t' \<noteq> t \<or> k' \<noteq> k \<longrightarrow> wtxn_state (svrs s' svr) t' k' = wtxn_state (svrs s svr) t' k') \<and>
-    rtxn_state (svrs s' svr) = rtxn_state (svrs s svr) \<and>
+definition prepare_write :: "svr_id \<Rightarrow> txid0 \<Rightarrow> 'v \<Rightarrow> tstmp \<Rightarrow> 'v state \<Rightarrow> 'v state \<Rightarrow> bool" where
+  "prepare_write svr t v gst_ts s s' \<equiv>
+    tid_match s t \<and>
+    (\<exists>kv_map.
+      txn_state (cls s (get_cl_txn t)) = WtxnPrep kv_map \<and> svr \<in> dom kv_map \<and> kv_map svr = Some v) \<and>
+    gst_ts =  (gst (cls s (get_cl_txn t))) \<and>
+    wtxn_state (svrs s svr) t = Ready \<and>
+    wtxn_state (svrs s' svr) t = Prep (clock (svrs s' svr)) (length (DS (svrs s svr))) \<and>
     clock (svrs s' svr) = Suc (clock (svrs s svr)) \<and>
     lst (svrs s' svr) = lst (svrs s svr) \<and>
     pending_wtxns (svrs s' svr) t = Some (clock (svrs s svr)) \<and>
-    (\<forall>t'. t' \<noteq> t \<longrightarrow> pending_wtxns (svrs s' svr) t' = pending_wtxns (svrs s svr) t') \<and>
-    DS (svrs s' svr) k = DS (svrs s svr) k @
+    DS (svrs s' svr) = DS (svrs s svr) @
       [\<lparr>v_value = v, v_writer = Tn t, v_readerset = {}, v_ts = clock (svrs s svr),
        v_gst = gst_ts, v_is_pending = True\<rparr>] \<and>
-    (\<forall>k'. k' \<noteq> k \<longrightarrow> DS (svrs s' svr) k' = DS (svrs s svr) k') \<and>
-    cls s' = cls s"
+    cls_svr_k'_t'_unchanged t svr s s'"
 
-fun find_and_commit :: "'v ep_version list \<Rightarrow> txid \<Rightarrow> tstmp \<Rightarrow> 'v ep_version list" where
-  "find_and_commit [] t commit_t = []" |
-  "find_and_commit (v # vl) t commit_t =
-    (if v_writer v = t then
-      v \<lparr>v_ts := commit_t, v_is_pending := False\<rparr> # vl
-    else v # (find_and_commit vl t commit_t))"
-
-definition commit_write :: "svr_id \<Rightarrow> txid0 \<Rightarrow> key \<Rightarrow> 'v state \<Rightarrow> 'v state \<Rightarrow> bool" where
-  "commit_write svr t k s s' \<equiv> \<exists>kv_map commit_t.
-    txn_state (cls s (get_cl_txn t)) = WtxnCommit commit_t kv_map \<and> k \<in> dom kv_map \<and>
-    loc k = svr \<and>
-    (\<exists>prep_t. wtxn_state (svrs s svr) t k = Prep prep_t) \<and>
-    wtxn_state (svrs s' svr) t k = Commit \<and>
-    (\<forall>t' k'. t' \<noteq> t \<or> k' \<noteq> k \<longrightarrow> wtxn_state (svrs s' svr) t' k' = wtxn_state (svrs s svr) t' k) \<and>
-    rtxn_state (svrs s' svr) = rtxn_state (svrs s svr) \<and>
+definition commit_write :: "svr_id \<Rightarrow> txid0 \<Rightarrow> 'v state \<Rightarrow> 'v state \<Rightarrow> bool" where
+  "commit_write svr t s s' \<equiv>
+    tid_match s t \<and>
+    (\<exists>kv_map commit_t.
+      txn_state (cls s (get_cl_txn t)) = WtxnCommit commit_t kv_map \<and> svr \<in> dom kv_map \<and>
+      (\<exists>prep_t i. wtxn_state (svrs s svr) t = Prep prep_t i \<and>
+       DS (svrs s' svr) = commit_in_vl (DS (svrs s svr)) commit_t i)) \<and>
+    wtxn_state (svrs s' svr) t = Commit \<and>
     clock (svrs s' svr) = clock (svrs s svr) \<and>
     lst (svrs s' svr) =
       (if dom (pending_wtxns (svrs s' svr)) = {} then clock (svrs s svr)
        else Min (ran (pending_wtxns (svrs s' svr)))) \<and>
     pending_wtxns (svrs s' svr) t = None \<and>
-    (\<forall>t'. t' \<noteq> t \<longrightarrow> pending_wtxns (svrs s' svr) t' = pending_wtxns (svrs s svr) t') \<and>
-    DS (svrs s' svr) k = find_and_commit (DS (svrs s svr) k) (Tn t) commit_t \<and>
-    (\<forall>k'. k' \<noteq> k \<longrightarrow> DS (svrs s' svr) k' = DS (svrs s svr) k')"
+    cls_svr_k'_t'_unchanged t svr s s'"
 
 subsubsection \<open>The Event System\<close>
 
@@ -241,24 +249,23 @@ definition state_init :: "'v state" where
                   gst = 0,
                   lst_map = (\<lambda>svr. 0),
                   cl_view = view_init \<rparr>),
-    svrs = (\<lambda>svr. \<lparr> wtxn_state = (\<lambda>t k. Ready),
-                    rtxn_state = (\<lambda>t k. NotReg),
+    svrs = (\<lambda>svr. \<lparr> wtxn_state = (\<lambda>t. Ready),
                     clock = 0,
                     lst = 0,
                     pending_wtxns = Map.empty,
-                    DS = DS_init \<rparr>)
+                    DS = DS_vl_init \<rparr>)
   \<rparr>"
 
 fun state_trans :: "'v state \<Rightarrow> 'v ev \<Rightarrow> 'v state \<Rightarrow> bool" where
-  "state_trans s (RInvoke cl keys sn u F) s' \<longleftrightarrow> read_invoke cl keys sn u F s s'" |
+  "state_trans s (RInvoke cl keys)        s' \<longleftrightarrow> read_invoke cl keys s s'" |
   "state_trans s (Read cl k v)            s' \<longleftrightarrow> read cl k v s s'" |
-  "state_trans s (RDone cl kv_map)        s' \<longleftrightarrow> read_done cl kv_map s s'" |
+  "state_trans s (RDone cl kv_map sn u)   s' \<longleftrightarrow> read_done cl kv_map sn u s s'" |
   "state_trans s (WInvoke cl kv_map)      s' \<longleftrightarrow> write_invoke cl kv_map s s'" |
-  "state_trans s (WCommit cl kv_map cts sn u F)  s' \<longleftrightarrow> write_commit cl kv_map cts sn u F s s'" |
+  "state_trans s (WCommit cl kv_map cts sn u)  s' \<longleftrightarrow> write_commit cl kv_map cts sn u s s'" |
   "state_trans s (WDone cl)               s' \<longleftrightarrow> write_done cl s s'" |
-  "state_trans s (RegR svr t k v i gts)   s' \<longleftrightarrow> register_read svr t k v i gts s s'" |
-  "state_trans s (PrepW svr t k v gts)    s' \<longleftrightarrow> prepare_write svr t k v gts s s'" |
-  "state_trans s (CommitW svr t k)        s' \<longleftrightarrow> commit_write svr t k s s'" |
+  "state_trans s (RegR svr t v i gts)     s' \<longleftrightarrow> register_read svr t v i gts s s'" |
+  "state_trans s (PrepW svr t v gts)      s' \<longleftrightarrow> prepare_write svr t v gts s s'" |
+  "state_trans s (CommitW svr t)          s' \<longleftrightarrow> commit_write svr t s s'" |
   "state_trans s Skip2 s' \<longleftrightarrow> s' = s"
 
 definition tps :: "('v ev, 'v state) ES" where
@@ -282,7 +289,7 @@ definition get_ver :: "'v ep_version \<Rightarrow> 'v version" where
 
 \<comment> \<open>TODO: define this properly\<close>
 definition kvs_of_s :: "'v state \<Rightarrow> 'v kv_store" where
-  "kvs_of_s s = (\<lambda>k. map get_ver (DS (svrs s (loc k)) k))"
+  "kvs_of_s s = (\<lambda>k. map get_ver (DS (svrs s k)))"
 
 definition views_of_s :: "'v state \<Rightarrow> (cl_id \<Rightarrow> view)" where
   "views_of_s s = (\<lambda>cl. cl_view (cls s cl))"
@@ -296,7 +303,7 @@ lemmas sim_defs = sim_def kvs_of_s_def views_of_s_def
 
 \<comment> \<open>Mediator function\<close>
 fun med :: "'v ev \<Rightarrow> 'v label" where
-  "med (RInvoke cl _ sn u F) = ET cl sn u F" |
-  "med (WCommit cl _ _ sn u F) = ET cl sn u F" |
+  "med (RDone cl kv_map sn u) = ET cl sn u (\<lambda>k op. case op of R \<Rightarrow> kv_map k | W \<Rightarrow> None)" |
+  "med (WCommit cl kv_map _ sn u) = ET cl sn u (\<lambda>k op. case op of R \<Rightarrow> None | W \<Rightarrow> kv_map k)" |
   "med _ = ETSkip"
 
